verif/verif_isvalid.v
@@ -24,13 +24,16 @@ Proof.
   forward_call(r,pr,c,pc).      (* t'2=currNode *)
   unfold cursor_correct_rel in H0.
   apply cursor_subnode in H0.
+  (* assert(subnode (currNode c r) (get_root r)) by auto. *)
   unfold relation_rep.
   destruct r as [[[root numRec] depth] prel]. autorewrite with norm.
   pose (r:=(root,numRec,depth,prel)).
-  Intros proot. rewrite subnode_rep with (n:=currNode c (root,numRec,depth,prel)) by auto.
-  Intros pcurr. subst. rewrite btnode_rep_getval at 1. normalize.
+  Intros proot. rewrite btnode_rep_getval. Intros.
+  rewrite subnode_rep with (n:=currNode c (root,numRec,depth,prel)) by auto.
+  Intros pcurr. subst prel. rewrite btnode_rep_getval at 1. normalize.
   pose (pcurr:=(getval (currNode c (root, numRec, depth, pr)))).
   rewrite unfold_btnode_rep at 1. fold pcurr.
+  assert(currNode c r = currNode c (root,numRec,depth,pr)). auto.
   destruct (currNode c (root,numRec,depth,pr)) as [ptr0 le b First Last x]. Intros.
   pose (currnode:= btnode val ptr0 le b First Last x).
   forward.                      (* t'5=t'2->numKeys *)
@@ -40,7 +43,7 @@ Proof.
      (PROP ( )
      LOCAL (temp _t'5 (Vint (Int.repr (Z.of_nat (numKeys (btnode val ptr0 le b First Last x)))));
             temp _t'2 pcurr; temp _t'1 (rep_index (entryIndex c)); temp _cursor pc;
-            temp _t'3 (Val.of_bool (isValid c)) (* new local *)
+            temp _t'3 (Val.of_bool (negb (isValid c r))) (* new local *)
            )
      SEP (field_at Tsh trelation [StructField _root] proot pr; malloc_token Tsh tbtnode pcurr;
      field_at Tsh tbtnode [StructField _numKeys]
@@ -59,11 +62,76 @@ Proof.
      malloc_token Tsh trelation pr; cursor_rep c (root, numRec, depth, pr) pc; emp)))%assert.
 
   - forward_call(r,pr,c,pc).
-    + admit.
-    + admit.
+    + unfold r. cancel. unfold relation_rep. Exists proot.
+      normalize. cancel. rewrite fold_btnode_rep by auto.
+      change_compspecs btrees.CompSpecs. (* TODO *)
+      cancel. eapply derives_trans. apply wand_frame_elim. cancel.
+    + unfold relation_rep. unfold r. Intros proot'. rewrite btnode_rep_getval. Intros.
+      rewrite <- H1 in H0. unfold get_root in H0. simpl in H0.
+      rewrite subnode_rep with (n:=currNode c r) by auto.
+      rewrite H1. Intros pn.
+      fold r. rewrite H1. unfold getval.
+      rewrite unfold_btnode_rep at 1.
+      Intros. subst pn.
+      forward.                  (* t'6=t'4->LastLeaf *)
+      * autorewrite with norm. entailer!. unfold is_int. destruct Last; simpl; auto.
+      * forward.                (* t'3=(tbool) (t'6==1) *)
+        entailer!.
+        { unfold isValid.
+          rewrite H1. destruct Last; simpl; auto.
+          destruct (index.index_eqb (entryIndex c) (index.ip (numKeys_le le))) eqn:eqb; simpl; auto.
+          admit.                (* there is a contradiction *)
+        }          
+        subst pcurr. cancel. cancel.
+        apply derives_refl.
   - forward.                    (* t'3=0 *)
-    admit.
-  - admit.
+    entailer!.
+    unfold isValid. rewrite H1.
+    destruct Last; auto.
+    assert(index.index_eqb (entryIndex c) (index.ip (numKeys_le le)) = false).
+    { unfold index.index_eqb.
+      (* this comes from the hypothesis H2 *)
+      unfold force_val in H5.
+      (* destruct (both_int (fun n1 n2 : int => Some (Val.of_bool (Int.eq n1 n2))) sem_cast_pointer sem_cast_pointer (rep_index (entryIndex c)) (Vint (Int.repr (Z.of_nat (numKeys_le le))))) eqn:both_int; inv H5. *)
+      destruct (entryIndex c); auto.
+      destruct((n =? numKeys_le le)%nat) eqn:eq; auto.
+      admit.                    (* there is a contradiction *)
+    } 
+    rewrite H2. auto.    
+    apply derives_refl.
+  - forward_if.
+    + forward. Exists (getval root).
+      eapply derives_trans.
+      assert (numKeys_le le = numKeys (btnode val ptr0 le b First Last x)). auto.
+      rewrite H2.
+      rewrite fold_btnode_rep by auto.
+      repeat rewrite sepcon_assoc. rewrite sepcon_comm. rewrite sepcon_comm. rewrite sepcon_comm.
+      repeat rewrite <- sepcon_assoc.
+      rewrite fold_btnode_rep by auto.
+      rewrite wand_sepcon_adjoint. rewrite wand_sepcon_adjoint. rewrite wand_sepcon_adjoint.
+      rewrite wand_sepcon_adjoint. rewrite wand_sepcon_adjoint.
+      eapply derives_trans. apply wand_frame_elim.
+      rewrite <- wand_sepcon_adjoint. rewrite <- wand_sepcon_adjoint. rewrite <- wand_sepcon_adjoint.
+      rewrite <- wand_sepcon_adjoint. rewrite <- wand_sepcon_adjoint.
+      apply derives_refl.
+      entailer!. fold r. rewrite H3. auto.
+      apply derives_refl.
+    + forward. Exists (getval root).
+      eapply derives_trans.
+      assert (numKeys_le le = numKeys (btnode val ptr0 le b First Last x)). auto.
+      rewrite H2.
+      rewrite fold_btnode_rep by auto.
+      repeat rewrite sepcon_assoc. rewrite sepcon_comm. rewrite sepcon_comm. rewrite sepcon_comm.
+      repeat rewrite <- sepcon_assoc.
+      rewrite fold_btnode_rep by auto.
+      rewrite wand_sepcon_adjoint. rewrite wand_sepcon_adjoint. rewrite wand_sepcon_adjoint.
+      rewrite wand_sepcon_adjoint. rewrite wand_sepcon_adjoint.
+      eapply derives_trans. apply wand_frame_elim.
+      rewrite <- wand_sepcon_adjoint. rewrite <- wand_sepcon_adjoint. rewrite <- wand_sepcon_adjoint.
+      rewrite <- wand_sepcon_adjoint. rewrite <- wand_sepcon_adjoint.
+      apply derives_refl.
+      entailer!. fold r. rewrite H3. auto.
+      apply derives_refl.
 Admitted.
   
 Lemma body_RL_CursorIsValid: semax_body Vprog Gprog f_RL_CursorIsValid RL_CursorIsValid_spec.
